%! Author = masprime77
%! Date = 25/11/2024

% Preamble
\documentclass[11pt]{article}

% Packages
\usepackage{amsmath}

% Document
\begin{document}
    \begin{1.6}
        \begin{gather*}
            \int_{-1}^{0} a(1+x) \, dx + \int_{0}^{1} a(1-x) \, dx = 1\\
            a \left( \int_{-1}^{0} 1+x \, dx + \int_{0}^{1} 1-x \, dx \right) = 1\\
            a\left( \left( [x]_{-1}^{0} + \left[ \frac{1}{2} x^{2} \right]_{-1}^{0} \right) + \left(  [x]_{0}^{1} + \left[ \frac{1}{2} x^{2} \right]_{0}^{1}  \right) \right) = 1 \\
            a(0 - (-1) + 0- \frac{1}{2} + 1 - 0 - (\frac{1}{2} - 0)) = 1 \\
            a(1 - \frac{1}{2} + 1 - \frac{1}{2}) = 1 \\
            a(1) = 1 \\
            a = 1 \\
        \end{gather*}
    \end{1.6}
\end{document}